x86model/Model/DecodeBi.v
@@ -108,6 +108,8 @@ Set Implicit Arguments.
 
   Definition op_s := "01100110".
 
+  Definition op_override_b: wf_bigrammar bool_t.
+
   Definition op_override_env : AST_Env bool_t :=
     {{0, ! op_s, (fun _ => true %% bool_t)}} :::
     {{1, ! (op_s ++ op_s), (fun _ => true %% bool_t)}} :::
